
\begin{tabular}{l|l|l}
    \multicolumn{3}{c}{Тригонометрические функции} \\
    \hline
    
    $\displaystyle sin^2(x) + cos^2(x) = 1$  & 
    $\displaystyle tg^2(x) + 1 = \frac{1}{cos^2(x)}$ &
    $\displaystyle tg(x) = \frac{sin(x)}{cos(x)}$ \\
    
    $\displaystyle tg(x)ctg(x) = 1$ &
    $\displaystyle ctg^2(x) + 1 = \frac{1}{sin^2(x)}$ &
    $\displaystyle ctg(x) = \frac{cos(x)}{x}$ \\  
    \hline
    
    $\displaystyle sin(x \pm y) = sin(x)cos(y) \pm cos(x)sin(y)$ & 
    $\displaystyle sin(x) = \frac{2tg\left(\frac{x}{2}\right)}{1 + tg^2\left(\frac{x}{2}\right)}$ &
    $\displaystyle sin(2x) = 2sin(x)cos(x)$ \\
    
    $\displaystyle cos(x \pm y) = cos(x)cos(y) \mp sin(x)sin(y)$ & 
    $\displaystyle cos(x) = \frac{1 - tg^2\left(\frac{x}{2}\right)}{1 + tg^2\left(\frac{x}{2}\right)}$ &
    $\displaystyle cos(2x) = cos^2(x) - sin^2(x)$ \\
    
    $\displaystyle tg(x \pm y) = \frac{tg(x) \pm tg(y)}{1 \mp tg(x)tg(y)}$ & 
    $\displaystyle tg(x) = \frac{2tg\left(\frac{x}{2}\right)}{1 - tg^2\left(\frac{x}{2}\right)}$ &
    $\displaystyle tg(2x) = \frac{2tg(x)}{1-tg^2(x)}$ \\
    
    $\displaystyle ctg(x \pm y) = \frac{-1 \pm ctg(x)ctg(y)}{ctg(x) \pm ctg(y)}$ & 
    $\displaystyle ctg(x) = \frac{1 - tg^2\left(\frac{x}{2}\right)}{2tg\left(\frac{x}{2}\right)}$ &
    $\displaystyle ctg(2x) = \frac{ctg^2(x) - 1}{2ctg(x)}$ \\
    \hline
    
    $\displaystyle sin(x) \pm sin(y) = 2sin\left(\frac{x \pm  y}{2}\right)cos\left(\frac{x \pm y}{2}\right)$ &
    $\displaystyle sin\left(\frac{x}{2}\right) = \sqrt{\frac{1 - cos(x)}{2}}$ &
    $\displaystyle sin^2(x) = \frac{1 - cos(2x)}{2}$ \\ 
    
    $\displaystyle cos(x) + cos(y) = 2cos\left(\frac{x +  y}{2}\right)cos\left(\frac{x - y}{2}\right)$ &
    $\displaystyle cos\left(\frac{x}{2}\right) = \sqrt{\frac{1 + cos(x)}{2}}$ &
    $\displaystyle cos^2(x) = \frac{1 + cos(2x)}{2}$ \\  
    
    $\displaystyle sin(x) \pm sin(y) = 2sin\left(\frac{x \pm  y}{2}\right)cos\left(\frac{x \pm y}{2}\right)$ &
    $\displaystyle tg\left(\frac{x}{2}\right) = \sqrt{\frac{1 - cos(x)}{1 + cos(x)}}$ &
    $\displaystyle (sin(x) + cos(x))^2 = 1 + sin(2x)$ \\  
    \hline
    
    $\displaystyle sin(x)sin(y) = \frac{1}{2}(cos(x - y) - cos(x + y))$ &
    $\displaystyle $ &
    $\displaystyle $ \\  
    
    $\displaystyle cos(x)cos(y) = \frac{1}{2}(cos(x - y) + cos(x + y))$ &
    $\displaystyle $ &
    $\displaystyle $ \\  
    
    $\displaystyle sin(x)cos(y) = \frac{1}{2}(sin(x - y) + sin(x + y))$ &
    $\displaystyle $ &
    $\displaystyle $ \\  
    \hline
    
    %    $\displaystyle $ &
    %    $\displaystyle $ &
    %    $\displaystyle $ \\     
\end{tabular}